merge (PRF_DRBG unmerged)

src/FCF/Bernoulli.v.d
@@ -1,1 +1,1 @@
-Bernoulli.vo Bernoulli.glob Bernoulli.v.beautified: Bernoulli.v ./Crypto.vo ./RndNat.vo
+Bernoulli.vo Bernoulli.glob Bernoulli.v.beautified: Bernoulli.v ./Crypto.vo ./RndNat.vo ./NotationV1.vo
