src/FCF/DiffieHellman.v.d
@@ -1,1 +1,1 @@
-DiffieHellman.vo DiffieHellman.glob DiffieHellman.v.beautified: DiffieHellman.v ./Crypto.vo ./RndNat.vo ./GroupTheory.vo
+DiffieHellman.vo DiffieHellman.glob DiffieHellman.v.beautified: DiffieHellman.v ./FCF.vo ./RndNat.vo ./GroupTheory.vo
