src/FCF/DistRules.v.d
@@ -1,1 +1,1 @@
-DistRules.vo DistRules.glob DistRules.v.beautified: DistRules.v ./DistSem.vo ./Fold.vo ./SemEquiv.vo ./DetSem.vo
+DistRules.vo DistRules.glob DistRules.v.beautified: DistRules.v ./DistSem.vo ./Fold.vo ./SemEquiv.vo ./DetSem.vo ./NotationV1.vo
