src/FCF/DistSem.v.d
@@ -1,1 +1,1 @@
-DistSem.vo DistSem.glob DistSem.v.beautified: DistSem.v ./Comp.vo ./Rat.vo ./Fold.vo ./Blist.vo ./StdNat.vo
+DistSem.vo DistSem.glob DistSem.v.beautified: DistSem.v ./Comp.vo ./Rat.vo ./Fold.vo ./Blist.vo ./StdNat.vo ./NotationV1.vo
