src/FCF/DistTacs.v.d
@@ -1,1 +1,1 @@
-DistTacs.vo DistTacs.glob DistTacs.v.beautified: DistTacs.v ./Rat.vo ./Comp.vo ./DistRules.vo ./DistSem.vo ./StdNat.vo ./Fold.vo
+DistTacs.vo DistTacs.glob DistTacs.v.beautified: DistTacs.v ./Rat.vo ./Comp.vo ./DistRules.vo ./DistSem.vo ./StdNat.vo ./Fold.vo ./NotationV1.vo
