src/FCF/Encryption_PK.v.d
@@ -1,1 +1,1 @@
-Encryption_PK.vo Encryption_PK.glob Encryption_PK.v.beautified: Encryption_PK.v ./Crypto.vo
+Encryption_PK.vo Encryption_PK.glob Encryption_PK.v.beautified: Encryption_PK.v ./FCF.vo
