src/FCF/ProgramLogic.v.d
@@ -1,1 +1,1 @@
-ProgramLogic.vo ProgramLogic.glob ProgramLogic.v.beautified: ProgramLogic.v ./Crypto.vo ./Bernoulli.vo
+ProgramLogic.vo ProgramLogic.glob ProgramLogic.v.beautified: ProgramLogic.v ./Crypto.vo ./Bernoulli.vo ./NotationV1.vo
